Veritas.BinTreePtr.fsti
@@ -8,6 +8,10 @@ open Veritas.BinTree
  *)
 type ptrfn = (n:bin_tree_node) -> (c:bin_tree_dir) -> option (d:bin_tree_node{is_desc d (child c n)})
 
+let points_to (pf: ptrfn) (d: bin_tree_node) (a: bin_tree_node{is_proper_desc d a}): bool = 
+  let c = desc_dir d a in
+  Some? (pf a c) && d = Some?.v (pf a c) 
+
 (* Is d reachable from a following pf pointers *)
 val reachable (pf: ptrfn) (d a: bin_tree_node): Tot bool
 
@@ -26,11 +30,21 @@ let non_reachable_sym (pf: ptrfn) (a1 a2: bin_tree_node): bool =
 val lemma_reachable_reflexive (pf: ptrfn) (a: bin_tree_node):
   Lemma (reachable pf a a)
 
+val lemma_points_to_reachable (pf: ptrfn) 
+                              (d: bin_tree_node) 
+                              (a: bin_tree_node):
+  Lemma (requires (is_proper_desc d a /\ points_to pf d a))
+        (ensures (reachable pf d a))
+
 (* pdesc is a transitive relation *)
 val lemma_reachable_transitive (pf: ptrfn) (a b c: bin_tree_node):
   Lemma (requires (reachable pf a b /\ reachable pf b c))
         (ensures (reachable pf a c))
 
+(* previous node in the reachability path from d to a *)
+val prev_in_path (pf:ptrfn) (d: bin_tree_node) (a:bin_tree_node{reachable pf d a /\ d <> a}): 
+  Tot (d': bin_tree_node {is_proper_desc d d' /\ reachable pf d' a /\ points_to pf d d'})
+                                    
 (* 
  * if there is no c-pointer at node a, then any desc in that subtree is not 
  * reachable from a 
